feat!(Client API): Client Encrypt/Decrypt now take requests

src/api/dotnet/Client.cs
@@ -1,9 +1,10 @@
-
 using System;
 using System.IO;
+using System.Numerics;
 using System.Collections.Generic;
 using System.Linq;
 using CMMDefs;
+using KeyringDefs;
 using Dafny;
 using ibyteseq = Dafny.ISequence<byte>;
 using icharseq = Dafny.ISequence<char>;
@@ -15,35 +16,16 @@ namespace AWSEncryptionSDK
     public class Client {
 
         // TODO: Proper documentation
-        public static MemoryStream Encrypt(MemoryStream plaintext, CMM cmm, Dictionary<string, string> encryptionContext = null, ushort? algorithmSuiteID = null, uint? frameLength = null) {
-            if (algorithmSuiteID != null && !AlgorithmSuite.__default.VALID__IDS.Elements.Contains((ushort)algorithmSuiteID)) {
-                throw new ArgumentException("Invalid algorithmSuiteID: " + algorithmSuiteID.ToString());
-            }
-            ibyteseq dafnyPlaintext = DafnyFFI.SequenceFromMemoryStream(plaintext);
-    
-            // TODO: This isn't checking for nulls or any of the requirements on the Dafny method.
-            // See https://github.com/dafny-lang/dafny/issues/461.
+        public static MemoryStream Encrypt(EncryptRequest request) {
             // TODO: Might need a lock here if ANYTHING in the Dafny runtime isn't threadsafe!
-            var optAlgorithmSuiteID = algorithmSuiteID != null ? STL.Option<ushort>.create_Some((ushort)algorithmSuiteID) : STL.Option<ushort>.create_None();
-            var optFrameLength = frameLength != null ? STL.Option<uint>.create_Some((uint)frameLength) : STL.Option<uint>.create_None();
-            var dafnyEncryptionContext = encryptionContext != null ? STL.Option<encryptioncontext>.create_Some(ToDafnyEncryptionContext(encryptionContext)) : STL.Option<encryptioncontext>.create_None();
-            STL.Result<ibyteseq> result = ESDKClient.__default.Encrypt(
-                    dafnyPlaintext,
-                    cmm,
-                    dafnyEncryptionContext,
-                    optAlgorithmSuiteID,
-                    optFrameLength
-                    );
-    
+            STL.Result<ibyteseq> result = ESDKClient.__default.Encrypt(request.GetDafnyRequest());
             return DafnyFFI.MemoryStreamFromSequence(DafnyFFI.ExtractResult(result));
         }
   
         // TODO: Proper documentation
-        public static MemoryStream Decrypt(MemoryStream cyphertext, CMM cmm) {
-            ibyteseq dafnyPlaintext = DafnyFFI.SequenceFromMemoryStream(cyphertext);
-    
+        public static MemoryStream Decrypt(DecryptRequest request) {
             // TODO: Might need a lock here if ANYTHING in the Dafny runtime isn't threadsafe!
-            STL.Result<ibyteseq> result = ESDKClient.__default.Decrypt(dafnyPlaintext, cmm);
+            STL.Result<ibyteseq> result = ESDKClient.__default.Decrypt(request.GetDafnyRequest());
     
             return DafnyFFI.MemoryStreamFromSequence(DafnyFFI.ExtractResult(result));
         }
@@ -53,6 +35,73 @@ namespace AWSEncryptionSDK
             IEnumerable<Pair<ibyteseq, ibyteseq>> e = encryptionContext.Select(entry
                 => new Pair<ibyteseq, ibyteseq>(DafnyFFI.DafnyUTF8BytesFromString(entry.Key), DafnyFFI.DafnyUTF8BytesFromString(entry.Value)));
             return encryptioncontext.FromElements(e.ToArray());
+        }
+
+        public class EncryptRequest {
+            public MemoryStream plaintext { get; set;}
+            public CMM cmm { get; set;}
+            public Keyring keyring { get; set;}
+            //public int? plaintextLength { get; set;}
+            public Dictionary<string, string> encryptionContext{ get; set;} = new Dictionary<string, string>() ;
+            public ushort? algorithmSuiteID { get; set;}
+            public uint? frameLength { get; set;}
+
+            internal ESDKClient.EncryptRequest GetDafnyRequest() {
+                if (this.plaintext == null) {
+                    throw new ArgumentNullException("EncryptRequest.plaintext must not be null.");
+                } else if (this.cmm == null && this.keyring == null) {
+                    throw new ArgumentNullException("EncryptRequest.cmm and EncryptRequest.keyring cannot both be null.");
+                } else if (this.cmm != null && this.keyring != null) {
+                    throw new ArgumentException("EncryptRequest.keyring OR EncryptRequest.cmm must be set (not both).");
+                } else if (this.encryptionContext == null) {
+                    throw new ArgumentNullException("EncryptRequest.encryptionContext must not be null.");
+                } else if (this.algorithmSuiteID != null && !AlgorithmSuite.__default.VALID__IDS.Elements.Contains((ushort)this.algorithmSuiteID)) {
+                    throw new ArgumentException("Invalid algorithm suite.");
+                }
+
+                if (this.cmm == null) {
+                    this.cmm = CMMs.MakeDefaultCMM(this.keyring);
+                }
+
+                var dafnyPlaintext = ESDKClient.SequenceStreamUnion.create(DafnyFFI.SequenceFromMemoryStream(this.plaintext));
+                var optionalAlgID = this.algorithmSuiteID != null ? STL.Option<ushort>.create_Some((ushort)this.algorithmSuiteID) : STL.Option<ushort>.create_None();
+
+                return new ESDKClient.EncryptRequest{
+                    plaintext = dafnyPlaintext,
+                    cmm = this.cmm,
+                    plaintextLength = new BigInteger(dafnyPlaintext.bytes.Count),
+                    encryptionContext = ToDafnyEncryptionContext(this.encryptionContext),
+                    algorithmSuiteID = optionalAlgID,
+                    frameLength = this.frameLength != null ? STL.Option<uint>.create_Some((uint)this.frameLength) : STL.Option<uint>.create_None()
+                };
+            }
+        }
+        
+        public class DecryptRequest {
+            public MemoryStream message { get; set;}
+            public CMM cmm { get; set;}
+            public Keyring keyring { get; set;}
+
+            internal ESDKClient.DecryptRequest GetDafnyRequest() {
+                if (this.message == null) {
+                    throw new ArgumentNullException("DecryptRequest.message must not be null.");
+                } else if (this.cmm == null && this.keyring == null) {
+                    throw new ArgumentNullException("DecryptRequest.cmm and DecryptRequest.keyring cannot both be null.");
+                } else if (this.cmm != null && this.keyring != null) {
+                    throw new ArgumentException("DecryptRequest.keyring OR DecryptRequest.cmm must be set (not both).");
+                }
+
+                if (this.cmm == null) {
+                    this.cmm = CMMs.MakeDefaultCMM(this.keyring);
+                }
+
+                var dafnyMessage = ESDKClient.SequenceStreamUnion.create(DafnyFFI.SequenceFromMemoryStream(this.message));
+
+                return new ESDKClient.DecryptRequest{
+                    message = dafnyMessage,
+                    cmm = this.cmm
+                };
+            }
         }
     }
 }
