src/Util/Streams.dfy
@@ -9,16 +9,18 @@ module Streams {
     const data: seq<T>
     var pos: nat
 
-    predicate Valid() reads this, Repr
+    predicate Valid()
+      reads this, Repr
+      ensures Valid() ==> this in Repr
     {
-      Repr == {this} &&
+      this in Repr &&
       pos <= |data|
     }
 
-    constructor(s: seq<T>)
+    constructor (s: seq<T>)
       ensures pos == 0
       ensures data[..] == s
-      ensures Valid()
+      ensures Valid() && fresh(Repr)
     {
       data := s;
       pos := 0;
@@ -61,23 +63,23 @@ module Streams {
 
   class ByteReader {
     ghost var Repr: set<object>
-    var reader: SeqReader<uint8>
+    const reader: SeqReader<uint8>
 
     predicate Valid()
       reads this, Repr
+      ensures Valid() ==> this in Repr
     {
       this in Repr &&
-      (reader in Repr && reader.Repr <= Repr && reader.Valid())
+      reader in Repr && reader.Repr <= Repr && this !in reader.Repr && reader.Valid()
     }
 
-    constructor(s: seq<uint8>)
+    constructor (s: seq<uint8>)
       ensures reader.data == s
-      ensures fresh(Repr - {this})
-      ensures Valid()
+      ensures Valid() && fresh(Repr)
     {
       var mr := new SeqReader<uint8>(s);
       reader := mr;
-      Repr := {this} + {reader} + mr.Repr;
+      Repr := {this} + mr.Repr;
     }
 
     method ReadByte() returns (res: Result<uint8>)
@@ -181,14 +183,16 @@ module Streams {
     ghost var Repr: set<object>
     var data: seq<T>
 
-    predicate Valid() reads this, Repr
+    predicate Valid()
+      reads this, Repr
+      ensures Valid() ==> this in Repr
     {
-      Repr == {this}
+      this in Repr
     }
 
     constructor()
       ensures data == []
-      ensures Valid()
+      ensures Valid() && fresh(Repr)
     {
       data := [];
       Repr := {this};
@@ -210,23 +214,23 @@ module Streams {
 
   class ByteWriter {
     ghost var Repr: set<object>
-    var writer: SeqWriter<uint8>
+    const writer: SeqWriter<uint8>
 
     predicate Valid()
       reads this, Repr
+      ensures Valid() ==> this in Repr
     {
       this in Repr &&
-      (writer in Repr && writer.Repr <= Repr && writer.Valid())
+      writer in Repr && writer.Repr <= Repr && this !in writer.Repr && writer.Valid()
     }
 
     constructor()
       ensures writer.data == []
-      ensures fresh(Repr - {this})
-      ensures Valid()
+      ensures Valid() && fresh(Repr)
     {
       var mw := new SeqWriter<uint8>();
       writer := mw;
-      Repr := {this} + {writer} + mw.Repr;
+      Repr := {this} + mw.Repr;
     }
 
     method WriteByte(n: uint8) returns (r: nat)
