test/SDK/Client.dfy
@@ -31,7 +31,10 @@ module {:extern "TestClient"} TestClient {
     import UTF8
     import Client = ESDKClient
   
-    method EncryptDecryptTest(cmm: CMMDefs.CMM) requires cmm.Valid()
+    method EncryptDecryptTest(cmm: CMMDefs.CMM)
+      requires cmm.Valid()
+      modifies cmm.Repr
+      ensures cmm.Valid() && fresh(cmm.Repr - old(cmm.Repr))
     {
       var msg :- expect UTF8.Encode("hello");
       var keyA :- expect UTF8.Encode("keyA");
@@ -50,9 +53,13 @@ module {:extern "TestClient"} TestClient {
         }
         assert Msg.KVPairsLength(encryptionContext) < UINT16_LIMIT;
       }
-      var e :- expect Client.Encrypt(msg, cmm, Some(encryptionContext), None, None);
 
-      var d :- expect Client.Decrypt(e, cmm);
+      var encryptRequest := new Client.EncryptRequest.NonStreamWithCMM(msg, cmm);
+      encryptRequest.EncryptionContext(encryptionContext);
+      var e :- expect Client.Encrypt(encryptRequest);
+
+      var decryptRequest := new Client.DecryptRequest.NonStreamWithCMM(e, cmm);
+      var d :- expect Client.Decrypt(decryptRequest);
 
       expect msg == d;
     }
